

MATH358 - Advanced Calculus

Based on lectures from Winter 2026 by Prof. John Toth.
Notes by Louis Meunier

Contents

1	Differentiation	2
1.1	Aside on Tangent Planes	7
1.2	Clairault's Theorem	7

§1 DIFFERENTIATION

We say $\Omega \subset \mathbb{R}^n$ a *domain* if it is open and connected.

↪ **Definition 1.1** (Differentiation): Let $f = (f_1, \dots, f_m)^T : \Omega \rightarrow \mathbb{R}^m$, Ω a domain in \mathbb{R}^n and $f_j : \Omega \rightarrow \mathbb{R}$. We say f *differentiable* at $x_0 \in \Omega$ if there exists a linear map $L : \mathbb{R}^n \rightarrow \mathbb{R}^m$ such that

$$\lim_{x \rightarrow x_0} \frac{\|f(x) - f(x_0) - L(x - x_0)\|}{\|x - x_0\|} = 0.$$

Remark 1.1: Note that the first norm on \mathbb{R}^m , the second on \mathbb{R}^n .

Remark 1.2: In terms of ε, δ , the definition says that $\forall \varepsilon > 0, \exists \delta > 0$ such that if $x \in \Omega \cap B(x_0, \delta)$, then $\|f(x) - f(x_0) - L(x - x_0)\| < \varepsilon \|x - x_0\|$.

↪ **Theorem 1.1:** L as above is unique if it exists.

PROOF. Suppose $L_1 \neq L_2$ both satisfy the definition. Then, for all $\varepsilon > 0$, there exists $\delta > 0$ such that if $0 < \|x - x_0\| < \delta$, then

$$\begin{aligned} \|(L_1 - L_2)(x - x_0)\| &\leq \|f(x) - f(x_0) - L_1(x - x_0)\| + \|f(x) - f(x_0) - L_2(x - x_0)\| \\ &\leq \varepsilon \|x - x_0\|, \end{aligned}$$

by differentiability (and the previous remark). In particular, $\|(L_1 - L_2)u\| < \varepsilon$ for all unit vectors u , which implies $\|(L_1 - L_2)u\| = 0$ and thus $L_1 = L_2$. ■

↪ **Definition 1.2:** If f differentiable at x_0 , we'll write $Df(x_0) = L$ for the *differential* of f at x_0 .

↪ **Proposition 1.1:** f differentiable at x_0 implies f continuous at x_0 . In fact, f is Lipschitz at x_0 .

PROOF. Let $\delta > 0$ such that $\|x - x_0\| < \delta$ implies $\|f(x) - f(x_0) - Df(x_0)(x - x_0)\| < \|x - x_0\|$, which implies

$$\|f(x) - f(x_0)\| \leq \|Df(x_0)(x - x_0)\| + \|x - x_0\| \leq (\|L\| + 1)\|x - x_0\|,$$

which readily proves the statement. ■

↪ **Proposition 1.2:** f differentiable at a point x_0 iff each of its component functions are differentiable at x_0 .

↪ **Definition 1.3:** For $f : \Omega \subset \mathbb{R}^n \rightarrow \mathbb{R}^m$, define the *partial derivative*

$$\frac{\partial f_j}{\partial x_i}(x_1, \dots, x_m) := \lim_{h \rightarrow 0} \frac{[f_j(x_1, \dots, x_i + h, \dots, x_m) - f_j(x_1, \dots, x_i, \dots, x_m)]}{h},$$

if the limit exists.

↪ **Proposition 1.3:** Let $f : \Omega \subset \mathbb{R}^n \rightarrow \mathbb{R}^m$ be differentiable at x_0 . Then, $\frac{\partial f_j}{\partial x_i}(x_0)$ exists for each $i = 1, \dots, n$ and $j = 1, \dots, m$, and

$$L = Df(x_0) = \left(\frac{\partial f_j}{\partial x_i}(x_0) \right)_{\substack{1 \leq i \leq n \\ 1 \leq j \leq m}}.$$

We call this matrix the Jacobian or derivative of f at x_0 .

PROOF. Write $L = (a_{ji})$ in the standard basis e_1, \dots, e_n for \mathbb{R}^n . Let $\varepsilon > 0$, fix some i with $1 \leq i \leq n$, and set $x := x_0 + he_i$, with $|h| < \delta$ sufficiently small. By differentiability,

$$\frac{\|f(x) - f(x_0) - L(x - x_0)\|}{\|x - x_0\|} = \left(\sum_{j=1}^m \left[\frac{f_j(x) - f_j(x_0)}{h} - a_{ji} \right]^2 \right)^{1/2}.$$

Since the limit as $h \rightarrow 0$ of the above ratio must be zero, the limit of each term in the summation as $h \rightarrow 0$ must be zero as well (being a sum of nonnegative terms), i.e.

$$\lim_{h \rightarrow 0} \frac{f_j(x) - f_j(x_0)}{h} = a_{ji} \quad \forall j = 1, \dots, m.$$

But the limit on the left is just $\frac{\partial f_j}{\partial x_i}(x_0)$, which proves all of the claims in turn. ■

Remark 1.3: This proposition says that f differentiable at x_0 implies $\frac{\partial f_j}{\partial x_i}(x_0)$ exists for all i, j . The converse need not be true. Consider

$$f(x, y) := \begin{cases} \frac{xy}{\sqrt{x^2+y^2}} & (x, y) \neq 0 \\ 0 & \text{else} \end{cases}.$$

⊗ **Example 1.1:** Another counterexample as in the previous remark is the function

$$f(x, y) := \begin{cases} \frac{x^2 y}{x^2 + y^2} & (x, y) \neq (0, 0) \\ 0 & (x, y) = (0, 0) \end{cases}.$$

Claim 1: f continuous at $(0, 0)$. We have, for $(x, y) \neq (0, 0)$,

$$\begin{aligned} |f(x, y) - f(0, 0)| &= \left| \frac{x^2 y}{x^2 + y^2} \right| \\ &= \frac{x^2 |y|}{x^2 + y^2} \\ &\leq |y| \rightarrow 0 \text{ as } (x, y) \rightarrow (0, 0), \end{aligned}$$

so we have continuity indeed.

Claim 2: $\partial_x f, \partial_y f$ exist at the origin, and are equal to zero. Note that $f(x, 0) = 0$ for $x \neq 0$, and $f(0, 0) = 0$, so it follows that $\partial_x f(0, 0) = 0$. Similarly for $\partial_y f(0, 0)$.

Claim 3: f is not differentiable at $(0, 0)$. Suppose otherwise. Then, $L = Df(0, 0) = (0, 0)$, so

$$\begin{aligned} 0 &= \lim_{(x, y) \rightarrow (0, 0)} \frac{|f(x, y) - f(0, 0) - Df(0, 0)(x, y)|}{\|(x, y)\|} \\ &= \lim_{(x, y) \rightarrow (0, 0)} \frac{|f(x, y)|}{\|(x, y)\|} \\ &= \lim_{(x, y) \rightarrow (0, 0)} \frac{x^2 |y|}{(x^2 + y^2) \cdot \sqrt{x^2 + y^2}} \\ &= \lim_{(x, y) \rightarrow (0, 0)} \frac{x^2 |y|}{(x^2 + y^2)^{3/2}}. \end{aligned}$$

Suppose $y = x$ in the final term (i.e., we approach the limit on a diagonal), and $x > 0$, then this ratio simplifies

$$\frac{x^3}{(2x^2)^{3/2}} = \frac{1}{2^{3/2}} \neq 0,$$

so we have a contradiction.

We can get a partial converse, however, if we assume continuity.

↪ **Theorem 1.2:** Let $f = (f_1, \dots, f_m) : \Omega \subset \mathbb{R}^n \rightarrow \mathbb{R}^m$. Suppose each $\frac{\partial f_j}{\partial x_i}$ is continuous at some $x^0 \in \Omega$. Then, f is differentiable at x^0 .

PROOF. We use MVT, and suppose $n = 2, m = 1$ for simplicity of notation, so that $f : \Omega \subset \mathbb{R}^2 \rightarrow \mathbb{R}$. We write $x = (x_1, x_2) \in \Omega, x^0 = (x_1^0, x_2^0)$. Let $\varepsilon > 0$. By assumption, there exists a $\delta > 0$ such that

$$\|y - x^0\| < \delta \Rightarrow \left| \frac{\partial f}{\partial x_i}(y) - \frac{\partial f}{\partial x_i}(x^0) \right| \leq \frac{\varepsilon}{2}, \quad i = 1, 2.$$

We write

$$\begin{aligned} f(x) - f(x^0) &= f(x_1, x_2) - f(x_1^0, x_2) + f(x_1^0, x_2) - f(x_1^0, x_2^0) \\ (\text{MVT, coordinate-wise}) &= \frac{\partial f}{\partial x_1}(z_1, x_2)(x_1 - x_1^0) + \frac{\partial f}{\partial x_2}(x_1^0, z_2)(x_2 - x_2^0), \end{aligned}$$

for some z_1 between x_1 and x_1^0 and some z_2 between x_2 and x_2^0 . Thus,

$$\begin{aligned} f(x) - f(x^0) - Df(x^0)(x - x^0) &= f(x) - f(x^0) - (\partial_{x_1}f(x^0), \partial_{x_2}f(x^0)) \cdot (x - x^0) \\ &= \frac{\partial f}{\partial x_1}(z_1, x_2)(x_1 - x_1^0) + \frac{\partial f}{\partial x_2}(x_1^0, z_2)(x_2 - x_2^0) \\ &\quad - \frac{\partial f}{\partial x_1}(x^0)(x_1 - x_1^0) - \frac{\partial f}{\partial x_2}(x^0)(x_2 - x_2^0) \\ &= [\partial_{x_1}f(z_1, x_2) - \partial_{x_1}f(x_1^0, x_2^0)](x_1 - x_1^0) \\ &\quad + [\partial_{x_2}f(x_1^0, z_2) - \partial_{x_2}f(x_1^0, x_2^0)](x_2 - x_2^0). \end{aligned}$$

By choice of z_1, z_2 and for (x_1, x_2) in $B(x^0, \delta)$, we know $(z_1, x_2) \in B(x^0, \delta)$ and $(x_1^0, z_2) \in B(x^0, \delta)$ as well, so we can appeal to continuity. In addition, it's clear that $|x_i - x_i^0| \leq \|x - x^0\|$. Thus, using continuity, we find

$$|f(x) - f(x^0) - Df(x^0)(x - x^0)| \leq \left(\frac{\varepsilon}{2} + \frac{\varepsilon}{2} \right) \|x - x^0\| = \varepsilon \|x - x^0\|,$$

so dividing both sides by $\|x - x^0\|$ immediately gives the result. ■

↪ **Definition 1.4:** Suppose $f : \Omega \subset \mathbb{R}^n \rightarrow \mathbb{R}$ has continuous $\frac{\partial f}{\partial x_i}$ at all points in Ω . Then, we say f is *continuously differentiable* (in Ω), and we write $f \in C^1(\Omega)$.

Remark 1.4: Continuity of partial derivatives is sufficient, but not necessary, for differentiability. For instance,

$$f(x, y) = \begin{cases} \frac{x^2 y^2}{x^2 + y^4} & (x, y) \neq (0, 0) \\ 0 & (x, y) = (0, 0) \end{cases}.$$

One readily computes $\partial_x f(0, 0) = \partial_y f(0, 0) = 0$, but along the parabola $x = t^2, y = t$ ($t \neq 0$),

$$\partial_x f(t^2, t) = \frac{1}{2},$$

so $\partial_x f$ can't be continuous. However, f is still differentiable at $(0, 0)$: we claim $L = 0$, then

$$\frac{|f(x, y) - f(0, 0) - L(x, y)|}{\|(x, y)\|} = \frac{|f(x, y)|}{(x^2 + y^2)^{\frac{1}{2}}} = \frac{x^2 y^2}{(x^2 + y^4)(x^2 + y^2)^{\frac{1}{2}}} \leq \frac{y^2}{|x^2 + y^2|^{\frac{1}{2}}} \leq |y| \xrightarrow{(x, y) \rightarrow 0} 0.$$

↪ **Proposition 1.4** (Basic Properties of Differentiation):

1. If $f, g : \Omega \rightarrow \mathbb{R}^m$ both differentiable at $x^0 \in \Omega$, then so is $F = f + g$, and

$$D(f + g)(x^0) = Df(x^0) + Dg(x^0).$$

2. If $f, g : \Omega \rightarrow \mathbb{R}^m$ both differentiable at $x^0 \in \Omega$, then so is $F = fg : \Omega \rightarrow \mathbb{R}$, and

$$DF(x^0) = f(x^0)Dg(x^0) + g(x^0)Df(x^0).$$

3. $f, g : \Omega \rightarrow \mathbb{R}$ both differentiable at x^0 with $g(x^0) \neq 0$, then so is $F = \frac{f}{g}$, and

$$DF(x^0) = \frac{DF(x^0)}{g(x^0)} - \frac{f(x^0)Dg(x^0)}{g^2(x^0)}.$$

4. (Chain Rule) Given $f : \Omega \subset \mathbb{R}^n \rightarrow \tilde{\Omega} \subset \mathbb{R}^m$ and $g : \tilde{\Omega} \rightarrow \mathbb{R}^k$, with f differentiable at x^0 and g differentiable at $y^0 = f(x^0)$, then $H = g \circ f : \Omega \subset \mathbb{R}^n \rightarrow \mathbb{R}^k$ is differentiable at x^0 , and

$$DH(x^0) = Dg(y^0) \cdot Df(x^0),$$

in which one should read the “ \cdot ” as matrix multiplication.

PROOF. 1., 2., 3. left as an exercise. We prove 4., the Chain Rule, for it is realistically the most interesting. Set $L := Dg(y_0) \cdot Df(x_0)$, and we'll write $y = f(x)$ (so in particular $y_0 = f(x_0)$, as in the statement). We need to show

$$\lim_{x \rightarrow x_0} \frac{\|H(x) - H(x_0) - L(x - x_0)\|}{\|x - x_0\|} = 0.$$

Let us work the numerator:

$$\begin{aligned} H(x) - H(x_0) - L(x - x_0) &= g(y) - g(y_0) - Dg(y_0)Df(x_0)(x - x_0) \\ &= g(y) - g(y_0) - Dg(y_0)(y - y_0) \\ &\quad + Dg(y_0)(y - y_0) - Dg(y_0)Df(x_0)(x - x_0) \\ &= g(y) - g(y_0) - Dg(y_0)(y - y_0) \\ &\quad + Dg(y_0)(f(x) - f(x_0) - Df(x_0)(x - x_0)). \end{aligned}$$

This means

$$\begin{aligned} \|H(x) - H(x_0) - L(x - x_0)\| &\leq \overbrace{\|g(y) - g(y_0) - Dg(y_0)(y - y_0)\|}^{=: (A)} \\ &\quad + \overbrace{\|Dg(y_0)\| \|f(x) - f(x_0) - Df(x_0)(x - x_0)\|}^{=: (B)}. \end{aligned}$$

By differentiability of f at x_0 , $(B) \rightarrow 0$ as $\|x - x_0\| \rightarrow 0$. We also have that, since f differentiable it is Lipschitz continuous, there is some $C > 0$ such that for $\|x - x_0\|$ sufficiently small,

$$(A) = \|y - y_0\| \cdot \frac{(A)}{\|y - y_0\|} \leq C\|x - x_0\| \frac{A}{\|y - y_0\|}.$$

By differentiability of g , the ratio $\frac{\|A\|}{\|y - y_0\|} \rightarrow 0$ as $\|y - y_0\| \rightarrow 0$. By continuity of f , $\|y - y_0\| = \|f(x) - f(x_0)\|$ will become small as $\|x - x_0\| \rightarrow 0$, so that we have in all $\frac{A}{\|x - x_0\|} \rightarrow 0$ as $\|x - x_0\| \rightarrow 0$. ■

Exercise 1.1: Let f differentiable in \mathbb{R}^2 and $g(r, \theta) := (r \cos \theta, r \sin \theta)$ with $(r, \theta) \in (0, \infty) \times [0, 2\pi)$. Let $F(r, \theta) = f(g(r, \theta))$. Compute $\frac{\partial F}{\partial \theta}$ and $\frac{\partial F}{\partial r}$.

§1.1 Aside on Tangent Planes

Let $f : \Omega \subset \mathbb{R}^n \rightarrow \mathbb{R}$ differentiable on Ω . Then $Df(x) = \left(\frac{\partial f}{\partial x_1}(x), \dots, \frac{\partial f}{\partial x_n}(x) \right) =: \nabla f(x)$, called the *gradient* of f . Let $S := \{(x, z) \in \Omega \times \mathbb{R} : z = f(x)\}$ be the *graph* of f . Then, for $x^0 \in \mathbb{R}^n$,

$$T_{x^0}S = \left\{ (x, z) \in \mathbb{R}^n \times \mathbb{R} : z = f(x^0) + \sum_{j=1}^n \frac{\partial f}{\partial x_j}(x^0)(x_j - x_j^0) \right\}$$

is the *tangent plane* to S at x^0 .

To see this, let $v \in \mathbb{R}^n$ be a unit vector and $x \in \Omega$. Define $g(t) := f(x + tv)$ for $f : \Omega \rightarrow \mathbb{R}$ differentiable (for t sufficiently small, $x + tv$ remains in Ω by openness). We find

$$g'(t) = \langle \nabla f(x + tv), v \rangle$$

for t sufficiently small.

↪ **Proposition 1.5:** Suppose $\nabla f(x) \neq 0$. Then, $\nabla f(x)$ points in the direction of steepest increase of f .

PROOF. For v a unit vector, the *directional derivative* in the direction of v is $D_v f(x) = \langle \nabla f(x), v \rangle = \|\nabla f(x)\| \cos(\theta)$ where θ the angle between $\nabla f(x)$ and v . This is maximized when $\theta = 0$, i.e. when $v = \frac{\nabla f(x_0)}{\|\nabla f(x_0)\|}$. ■

We can rewrite the graph S as the level set $\{(x, z) \in \Omega \times \mathbb{R} \mid g(x, z) = 0\}$ where $g(x, z) := z - f(x)$. Heuristically, $\nabla g(x_0, z_0)$ should be *normal* to the surface S at (x_0, z_0) (for steepest increase). As such, we define

$$T_{(x_0, z_0)}S := \{\nabla g(x_0, z_0) \cdot (x - x_0, z - z_0) = 0\}.$$

Note that

$$\nabla g(x_0, z_0) = (-\partial_{x_1}f(x_0), \dots, -\partial_{x_n}f(x_0), 1),$$

so that

$$T_{(x_0, z_0)}S = \{z - z_0 = \nabla f(x_0) \cdot (x - x_0)\},$$

which gives the definition from above.

§1.2 Clairault's Theorem

Here, the question is, given $f : \Omega \subset \mathbb{R}^n \rightarrow \mathbb{R}$ twice differentiable, when can we exchange order of second-order partial derivatives, i.e. when is

$$\frac{\partial^2 f}{\partial x_j \partial x_i} = \frac{\partial^2 f}{\partial x_i \partial x_j}, \quad \forall i, j = 1, \dots, n?$$

We need to establish first a generalization of the mean-value theorem. First, note that if

$$\gamma : (a, b) \rightarrow \mathbb{R}^n, \quad g : \Omega \subset \mathbb{R}^n \rightarrow \mathbb{R}$$

are two differentiable functions with $\gamma((a, b)) \subset \Omega$, then by the chain rule, if we put $H(t) := g(\gamma(t))$,

$$\frac{\partial H}{\partial t} = Dg(\gamma(t)) \cdot D\gamma(t), \quad D\gamma(t) = (\gamma'_1(t), \dots, \gamma'_n(t)).$$

↪ **Theorem 1.3** (Mean-Value Theorem): Let $B \subset \mathbb{R}^n$ be a ball and $f : B \rightarrow \mathbb{R}$ be differentiable for all $x \in B$. Then, for any $x, y \in B$, there exists $z \in B$ such that

$$f(x) - f(y) = Df(z) \cdot (x - y).$$

In particular, $|f(x) - f(y)| \leq \|Df(z)\| \|x - y\|$.

PROOF. Let $x, y \in B$ fixed and let $\gamma(t) := tx + (1 - t)y$ for $t \in [0, 1]$. We see that $\gamma(t) \in B$ for all $t \in [0, 1]$, and that $D\gamma(t) = x - y$. Set $F(t) := f(\gamma(t))$ (i.e., we restrict f to its values along the straight line along x and y), noting $F : \mathbb{R} \rightarrow \mathbb{R}$. So, by 1-dimensional mean-value theorem, there is some $t^* \in [0, 1]$ such that

$$\begin{aligned} f(x) - f(y) &= F(1) - F(0) = F'(t^*) = Df\left(\underbrace{t^*x + (1 - t^*)y}_{=: z \in B}\right) \cdot D\gamma(t) \\ &= Df(z) \cdot (x - y). \end{aligned}$$

■

Let $f : \Omega \subset \mathbb{R}^n \rightarrow \mathbb{R}^m$ differentiable. Remember that $Df : \Omega \rightarrow \mathbb{R}^{m \times n}$.

↪ **Definition 1.5**: We say f twice differentiable at x if Df exists locally to x and Df is differentiable at x . We write

$$D^2f = D(Df),$$

and similarly

$$D^k f := D(D^{k-1}f)$$

with an analogous definition.

↪ **Definition 1.6**: Given $f : \Omega \subset \mathbb{R}^n \rightarrow \mathbb{R}$, we see that $f \in C^k(\Omega)$ for $k \in \mathbb{Z}_+$ if all the partial derivatives to order k exist and are continuous in Ω .

↪ **Definition 1.7:** If $f : \Omega \subset \mathbb{R}^n \rightarrow \mathbb{R}$ twice differentiable, the *Hessian matrix* is given by

$$H_f(x) = \begin{pmatrix} \frac{\partial^2 f}{\partial x_1 \partial x_1} & \frac{\partial^2 f}{\partial x_1 \partial x_2} & \cdots & \frac{\partial^2 f}{\partial x_1 \partial x_n} \\ \vdots & \vdots & \ddots & \vdots \\ \frac{\partial^2 f}{\partial x_n \partial x_1} & \frac{\partial^2 f}{\partial x_n \partial x_2} & \cdots & \frac{\partial^2 f}{\partial x_n \partial x_n} \end{pmatrix}.$$

Exercise 1.2: Let $f(x, y) := \begin{cases} \frac{(xy)(x^2-y^2)}{x^2+y^2} & (x,y) \neq (0,0) \\ 0 & (x,y) = (0,0) \end{cases}$ and compute $H_f(x, y)$.

↪ **Theorem 1.4 (Clairault):** Let $f : \Omega \subset \mathbb{R}^n \rightarrow \mathbb{R}$ be twice differentiable at $x \in \Omega$. Then,

$$\frac{\partial^2 f}{\partial x_i \partial x_j}(x) = \frac{\partial^2 f}{\partial x_j \partial x_i}(x), \quad \forall i, j = 1, \dots, n.$$

↪ **Corollary 1.1:** If $\frac{\partial^2 f}{\partial x_i \partial x_j}$ are all continuous at $x \in \Omega$ for $i, j = 1, \dots, n$, then $\frac{\partial^2 f}{\partial x_i \partial x_j}(x) = \frac{\partial^2 f}{\partial x_j \partial x_i}(x)$.

PROOF. (Of Clairault's) It's enough to consider $n = 2$. Fix $(x, y) \in \Omega$, and note that for $s, t \in \mathbb{R}$ sufficiently small, $(x + s, y + t) \in \Omega$ by openness. Set

$$\begin{aligned} \Delta(s, t) &:= f(x + s, y + t) - f(x, y + t) - f(x + s, y) + f(x, y) \\ &= g_t(x + s) - g_t(x), \quad g_t(u) := f(u, y + t) - f(u, y). \end{aligned}$$

By the mean-value theorem, there is some $\xi_{s,t}$ between x and $x + s$ such that

$$\Delta(s, t) = \frac{\partial g_t}{\partial x}(\xi_{s,t}) \cdot s = \left[\frac{\partial f}{\partial x}(\xi_{s,t}, y + t) - \frac{\partial f}{\partial x}(\xi_{s,t}, y) \right] s. \quad (\dagger)$$

By assumption, $\frac{\partial f}{\partial x}$ is differentiable at (x, y) , so

$$\frac{\partial f}{\partial x}(z_1, z_2) = \frac{\partial f}{\partial x}(x, y)(z_1 - x) + \frac{\partial^2}{\partial x^2}(x, y)(z_2 - y) + E_1(z_1, z_2), \quad (\ddagger)$$

where

$$\frac{|E_1(z_1, z_2)|}{\sqrt{(z_1 - x)^2 + (z_2 - y)^2}} \rightarrow 0, \quad \text{as } (z_1, z_2) \rightarrow (x, y).$$

Evaluating (\ddagger) at $(z_1, z_2) = (\xi_{s,t}, y + t)$ and $(\xi_{s,t}, y)$, and plugging into (\dagger) yields

$$\Delta(s, t) = \left(\frac{\partial^2 f}{\partial y \partial x}(x, y)t + E_1(\xi_{s,t}, y + t) - E_1(\xi_{s,t}, y) \right) s.$$

Let $s = t$ and let $t \rightarrow 0$. We claim that

$$\frac{\partial^2 f}{\partial y \partial x}(x, y) = \lim_{s=t \rightarrow 0} \frac{\Delta(s, t)}{st} = \frac{\partial^2 f}{\partial x \partial y}(x, y)$$

■